examples/AutoSep.v
@@ -341,7 +341,7 @@ Ltac hints_ext_simplifier hints := fun s1 s2 s3 H =>
          provers.WordProver.pow32 provers.WordProver.wplus' provers.WordProver.wneg' provers.WordProver.wminus' wordBin NToWord Nplus minus
          provers.WordProver.decompose combine Expr.expr_seq_dec provers.WordProver.combineAll provers.WordProver.combine app
          provers.WordProver.alreadyCovered provers.WordProver.alreadyCovered' andb orb provers.WordProver.merge provers.WordProver.wordLearn1 provers.WordProver.wordLearn
-         provers.WordProver.equalitysEq ILEnv.W_seq weq provers.WordProver.equalityMatches provers.WordProver.wordProve provers.WordProver.wordSummarize
+         provers.WordProver.equalitysEq ILEnv.W_seq Word.weqb weq provers.WordProver.equalityMatches provers.WordProver.wordProve provers.WordProver.wordSummarize
          provers.WordProver.types ILEnv.bedrock_type_W provers.WordProver.zero Bool.bool_dec wzero' posToWord bool_rec bool_rect
          Nminus wordToN Nsucc Nmult Pos.mul Pos.add Pos.sub_mask Pos.succ_double_mask Pos.double_mask Pos.pred_double
          provers.WordProver.natToWord' mod2 Div2.div2 whd wtl Pos.double_pred_mask
@@ -401,6 +401,7 @@ Ltac hints_ext_simplifier hints := fun s1 s2 s3 H =>
          CANCEL.order_impures 
          CANCEL.cancel_in_order
          CANCEL.unify_remove CANCEL.unifyArgs
+         CANCEL.expr_size
 
          ILTac.canceller
          
@@ -704,7 +705,7 @@ Ltac hints_ext_simplifier hints := fun s1 s2 s3 H =>
          provers.WordProver.pow32 provers.WordProver.wplus' provers.WordProver.wneg' provers.WordProver.wminus' wordBin NToWord Nplus minus
          provers.WordProver.decompose combine Expr.expr_seq_dec provers.WordProver.combineAll provers.WordProver.combine app
          provers.WordProver.alreadyCovered provers.WordProver.alreadyCovered' andb orb provers.WordProver.merge provers.WordProver.wordLearn1 provers.WordProver.wordLearn
-         provers.WordProver.equalitysEq ILEnv.W_seq weq provers.WordProver.equalityMatches provers.WordProver.wordProve provers.WordProver.wordSummarize
+         provers.WordProver.equalitysEq ILEnv.W_seq Word.weqb weq provers.WordProver.equalityMatches provers.WordProver.wordProve provers.WordProver.wordSummarize
          provers.WordProver.types ILEnv.bedrock_type_W provers.WordProver.zero Bool.bool_dec wzero' posToWord bool_rec bool_rect
          Nminus wordToN Nsucc Nmult Pos.mul Pos.add Pos.sub_mask Pos.succ_double_mask Pos.double_mask Pos.pred_double
          provers.WordProver.natToWord' mod2 Div2.div2 whd wtl Pos.double_pred_mask
@@ -768,6 +769,7 @@ Ltac hints_ext_simplifier hints := fun s1 s2 s3 H =>
          CANCEL.order_impures 
          CANCEL.cancel_in_order
          CANCEL.unify_remove CANCEL.unifyArgs
+         CANCEL.expr_size
          
          ILTac.canceller
 
